src/ocaml-output/FStar_ToSyntax_ToSyntax.ml
@@ -227,18 +227,10 @@ let rec (is_comp_type :
       | FStar_Parser_AST.Name l when
           (let uu___1 = FStar_Syntax_DsEnv.current_module env in
            FStar_Ident.lid_equals uu___1 FStar_Parser_Const.prims_lid) &&
-            (let uu___1 =
-               let uu___2 = FStar_Ident.ident_of_lid l in
-               FStar_Ident.string_of_id uu___2 in
-             uu___1 = "Tot")
-          -> true
-      | FStar_Parser_AST.Name l when
-          (let uu___1 = FStar_Syntax_DsEnv.current_module env in
-           FStar_Ident.lid_equals uu___1 FStar_Parser_Const.prims_lid) &&
-            (let uu___1 =
-               let uu___2 = FStar_Ident.ident_of_lid l in
-               FStar_Ident.string_of_id uu___2 in
-             uu___1 = "GTot")
+            (let s =
+               let uu___1 = FStar_Ident.ident_of_lid l in
+               FStar_Ident.string_of_id uu___1 in
+             (s = "Tot") || (s = "GTot"))
           -> true
       | FStar_Parser_AST.Name l ->
           let uu___1 = FStar_Syntax_DsEnv.try_lookup_effect_name env l in
