src/ocaml-output/FStar_TypeChecker_Env.ml
@@ -5707,8 +5707,17 @@ let (print_gamma : FStar_Syntax_Syntax.gamma -> Prims.string) =
            (fun uu___1 ->
               match uu___1 with
               | FStar_Syntax_Syntax.Binding_var x ->
-                  let uu___2 = FStar_Syntax_Print.bv_to_string x in
-                  Prims.op_Hat "Binding_var " uu___2
+                  let uu___2 =
+                    let uu___3 = FStar_Syntax_Print.bv_to_string x in
+                    let uu___4 =
+                      let uu___5 =
+                        let uu___6 =
+                          FStar_Syntax_Print.term_to_string
+                            x.FStar_Syntax_Syntax.sort in
+                        Prims.op_Hat uu___6 ")" in
+                      Prims.op_Hat ":" uu___5 in
+                    Prims.op_Hat uu___3 uu___4 in
+                  Prims.op_Hat "Binding_var (" uu___2
               | FStar_Syntax_Syntax.Binding_univ u ->
                   let uu___2 = FStar_Ident.string_of_id u in
                   Prims.op_Hat "Binding_univ " uu___2
@@ -5716,6 +5725,21 @@ let (print_gamma : FStar_Syntax_Syntax.gamma -> Prims.string) =
                   let uu___3 = FStar_Ident.string_of_lid l in
                   Prims.op_Hat "Binding_lid " uu___3)) in
     FStar_Compiler_Effect.op_Bar_Greater uu___ (FStar_String.concat "::\n")
+let (is_contained_in :
+  FStar_Syntax_Syntax.gamma -> FStar_Syntax_Syntax.gamma -> Prims.bool) =
+  fun g1 ->
+    fun g2 ->
+      FStar_Compiler_List.for_all
+        (fun uu___ ->
+           match uu___ with
+           | FStar_Syntax_Syntax.Binding_var id1 ->
+               FStar_Compiler_List.existsb
+                 (fun uu___1 ->
+                    match uu___1 with
+                    | FStar_Syntax_Syntax.Binding_var id2 ->
+                        FStar_Syntax_Syntax.bv_eq id1 id2
+                    | uu___2 -> false) g2
+           | uu___1 -> true) g1
 let (string_of_delta_level : delta_level -> Prims.string) =
   fun uu___ ->
     match uu___ with
@@ -6272,7 +6296,9 @@ let (new_implicit_var_aux :
                     {
                       FStar_Syntax_Syntax.uvar_decoration_typ = k;
                       FStar_Syntax_Syntax.uvar_decoration_should_check =
-                        should_check
+                        should_check;
+                      FStar_Syntax_Syntax.uvar_decoration_solution_bs =
+                        FStar_Syntax_Syntax.Solution_gamma_unknown
                     } in
                   let ctx_uvar =
                     let uu___2 = FStar_Syntax_Unionfind.fresh decoration r in
