ulib/experimental/Steel.Effect.Common.fsti
@@ -41,6 +41,8 @@ irreducible let ite_attr : unit = ()
 unfold
 let true_p : prop = True
 
+module T = FStar.Tactics
+
 let join_preserves_interp (hp:slprop) (m0:hmem hp) (m1:mem{disjoint m0 m1})
 : Lemma
   (interp hp (join m0 m1))
@@ -2291,6 +2293,7 @@ let try_open_existentials () : Tac bool =
 
 /// Solves a `can_be_split` constraint
 let rec solve_can_be_split (args:list argv) : Tac bool =
+  // dump "Solve can be split";
   match args with
   | [(t1, _); (t2, _)] ->
       let lnbr = slterm_nbr_uvars t1 in
@@ -2318,6 +2321,7 @@ let rec solve_can_be_split (args:list argv) : Tac bool =
                               `%fst; `%snd];
                             delta_attr [`%__reduce__];
                             primops; iota; zeta];
+                       // dump "Calling canon";
                        canon' false (`true_p) (`true_p)));
           true
         with
